Introduce CompCert behaviors and simulations. Add a proof of LTT-PLTT behaviors preservation based on them.

Behavior.v
@@ -1,7 +1,9 @@
-(* from CompCert Behaviors.v *)
-
+Require Import Classical.
+Require Import ClassicalEpsilon.
+Require Import Coqlib.
 Require Import Events.
 Require Import Smallstep.
+
 Set Implicit Arguments.
 
 Inductive program_behavior: Type :=
@@ -10,13 +12,84 @@ Inductive program_behavior: Type :=
   | Reacts: traceinf -> program_behavior
   | Goes_wrong: trace -> program_behavior.
 
+(** Operations and relations on behaviors *)
+
+Definition not_wrong (beh: program_behavior) : Prop :=
+  match beh with
+  | Terminates _ => True
+  | Diverges _ => True
+  | Reacts _ => True
+  | Goes_wrong _ => False
+  end.
+
+Definition behavior_app (t: trace) (beh: program_behavior): program_behavior :=
+  match beh with
+  | Terminates t1 => Terminates (t ** t1)
+  | Diverges t1 => Diverges (t ** t1)
+  | Reacts T => Reacts (t *** T)
+  | Goes_wrong t1 => Goes_wrong (t ** t1)
+  end.
+
+Lemma behavior_app_assoc:
+  forall t1 t2 beh,
+  behavior_app (t1 ** t2) beh = behavior_app t1 (behavior_app t2 beh).
+Proof.
+  intros. destruct beh; simpl; f_equal; traceEq.
+Qed.
+
+Lemma behavior_app_E0:
+  forall beh, behavior_app E0 beh = beh.
+Proof.
+  destruct beh; auto.
+Qed.
+
+Definition behavior_prefix (t: trace) (beh: program_behavior) : Prop :=
+  exists beh', beh = behavior_app t beh'.
+
+Definition behavior_improves (beh1 beh2: program_behavior) : Prop :=
+  beh1 = beh2 \/ exists t, beh1 = Goes_wrong t /\ behavior_prefix t beh2.
+
+Lemma behavior_improves_refl:
+  forall beh, behavior_improves beh beh.
+Proof.
+  intros; red; auto.
+Qed.
+
+Lemma behavior_improves_trans:
+  forall beh1 beh2 beh3,
+  behavior_improves beh1 beh2 -> behavior_improves beh2 beh3 ->
+  behavior_improves beh1 beh3.
+Proof.
+  intros. red. destruct H; destruct H0; subst; auto.
+  destruct H as [t1 [EQ1 [beh2' EQ1']]].
+  destruct H0 as [t2 [EQ2 [beh3' EQ2']]].
+  subst. destruct beh2'; simpl in EQ2; try discriminate. inv EQ2.
+  right. exists t1; split; auto. exists (behavior_app t beh3'). apply behavior_app_assoc.
+Qed.
+
+Lemma behavior_improves_bot:
+  forall beh, behavior_improves (Goes_wrong E0) beh.
+Proof.
+  intros. right. exists E0; split; auto. exists beh. rewrite behavior_app_E0; auto.
+Qed.
+
+Lemma behavior_improves_app:
+  forall t beh1 beh2,
+  behavior_improves beh1 beh2 ->
+  behavior_improves (behavior_app t beh1) (behavior_app t beh2).
+Proof.
+  intros. red; destruct H. left; congruence.
+  destruct H as [t' [A [beh' B]]]. subst.
+  right; exists (t ** t'); split; auto. exists beh'. rewrite behavior_app_assoc; auto.
+Qed.
+
+(** Associating behaviors to programs. *)
 
 Section PROGRAM_BEHAVIORS.
-  
-  Variable L: semantics.
 
-  (* only removed the return value *)
-  Inductive state_behaves (s: state L): program_behavior -> Prop :=
+Variable L: semantics.
+
+Inductive state_behaves (s: state L): program_behavior -> Prop :=
   | state_terminates: forall t s',
       Star L s t s' ->
       final_state L s' ->
@@ -33,7 +106,7 @@ Section PROGRAM_BEHAVIORS.
       ~final_state L s' ->
       state_behaves s (Goes_wrong t).
 
-  Inductive program_behaves: program_behavior -> Prop :=
+Inductive program_behaves: program_behavior -> Prop :=
   | program_runs: forall s beh,
       initial_state L s -> state_behaves s beh ->
       program_behaves beh
@@ -41,4 +114,195 @@ Section PROGRAM_BEHAVIORS.
       (forall s, ~initial_state L s) ->
       program_behaves (Goes_wrong E0).
 
+Lemma state_behaves_app:
+  forall s1 t s2 beh,
+  Star L s1 t s2 -> state_behaves s2 beh -> state_behaves s1 (behavior_app t beh).
+Proof.
+  intros. inv H0; simpl; econstructor; eauto; try (eapply star_trans; eauto).
+  eapply star_forever_reactive; eauto.
+Qed.
+
+(** * Existence of behaviors *)
+
+Section TRACEINF_REACTS.
+
+Variable s0: state L.
+
+Hypothesis reacts:
+  forall s1 t1, Star L s0 t1 s1 ->
+  exists s2, exists t2, Star L s1 t2 s2 /\ t2 <> E0.
+
+Lemma reacts':
+  forall s1 t1, Star L s0 t1 s1 ->
+  { s2 : state L & { t2 : trace | Star L s1 t2 s2 /\ t2 <> E0 } }.
+Proof.
+  intros.
+  destruct (constructive_indefinite_description _ (reacts H)) as [s2 A].
+  destruct (constructive_indefinite_description _ A) as [t2 [B C]].
+  exists s2; exists t2; auto.
+Qed.
+
+CoFixpoint build_traceinf' (s1: state L) (t1: trace) (ST: Star L s0 t1 s1) : traceinf' :=
+  match reacts' ST with
+  | existT s2 (exist t2 (conj A B)) =>
+      Econsinf' t2
+                (build_traceinf' (star_trans ST A (refl_equal _)))
+                B
+  end.
+
+Lemma reacts_forever_reactive_rec:
+  forall s1 t1 (ST: Star L s0 t1 s1),
+  Forever_reactive L s1 (traceinf_of_traceinf' (build_traceinf' ST)).
+Proof.
+  cofix COINDHYP; intros.
+  rewrite (unroll_traceinf' (build_traceinf' ST)). simpl.
+  destruct (reacts' ST) as [s2 [t2 [A B]]].
+  rewrite traceinf_traceinf'_app.
+  econstructor. eexact A. auto. apply COINDHYP.
+Qed.
+
+Lemma reacts_forever_reactive:
+  exists T, Forever_reactive L s0 T.
+Proof.
+  exists (traceinf_of_traceinf' (build_traceinf' (star_refl (step L) (globalenv L) s0))).
+  apply reacts_forever_reactive_rec.
+Qed.
+
+End TRACEINF_REACTS.
+
+Lemma diverges_forever_silent:
+  forall s0,
+  (forall s1 t1, Star L s0 t1 s1 -> exists s2, Step L s1 E0 s2) ->
+  Forever_silent L s0.
+Proof.
+  cofix COINDHYP; intros.
+  destruct (H s0 E0) as [s1 ST]. constructor.
+  econstructor. eexact ST. apply COINDHYP.
+  intros. eapply H. eapply star_left; eauto.
+Qed.
+
+Lemma state_behaves_exists:
+  forall s, exists beh, state_behaves s beh.
+Proof.
+  intros s0.
+  destruct (classic (forall s1 t1, Star L s0 t1 s1 -> exists s2, exists t2, Step L s1 t2 s2)).
+(* 1 Divergence (silent or reactive) *)
+  destruct (classic (exists s1, exists t1, Star L s0 t1 s1 /\
+                       (forall s2 t2, Star L s1 t2 s2 ->
+                        exists s3, Step L s2 E0 s3))).
+(* 1.1 Silent divergence *)
+  destruct H0 as [s1 [t1 [A B]]].
+  exists (Diverges t1); econstructor; eauto.
+  apply diverges_forever_silent; auto.
+(* 1.2 Reactive divergence *)
+  destruct (@reacts_forever_reactive s0) as [T FR].
+  intros.
+  generalize (not_ex_all_not _ _ H0 s1). intro A; clear H0.
+  generalize (not_ex_all_not _ _ A t1). intro B; clear A.
+  destruct (not_and_or _ _ B). contradiction.
+  destruct (not_all_ex_not _ _ H0) as [s2 C]; clear H0.
+  destruct (not_all_ex_not _ _ C) as [t2 D]; clear C.
+  destruct (imply_to_and _ _ D) as [E F]; clear D.
+  destruct (H s2 (t1 ** t2)) as [s3 [t3 G]]. eapply star_trans; eauto.
+  exists s3; exists (t2 ** t3); split.
+  eapply star_right; eauto.
+  red; intros. destruct (app_eq_nil t2 t3 H0). subst. elim F. exists s3; auto.
+  exists (Reacts T); econstructor; eauto.
+(* 2 Termination (normal or by going wrong) *)
+  destruct (not_all_ex_not _ _ H) as [s1 A]; clear H.
+  destruct (not_all_ex_not _ _ A) as [t1 B]; clear A.
+  destruct (imply_to_and _ _ B) as [C D]; clear B.
+  destruct (classic (final_state L s1)) as [FINAL | NOTFINAL].
+(* 2.1 Normal termination *)
+  exists (Terminates t1); econstructor; eauto.
+(* 2.2 Going wrong *)
+  exists (Goes_wrong t1); econstructor; eauto. red. intros.
+  generalize (not_ex_all_not _ _ D s'); intros.
+  generalize (not_ex_all_not _ _ H t); intros.
+  auto.
+Qed.
+
+Theorem program_behaves_exists:
+  exists beh, program_behaves beh.
+Proof.
+  destruct (classic (exists s, initial_state L s)) as [[s0 INIT] | NOTINIT].
+(* 1. Initial state is defined. *)
+  destruct (state_behaves_exists s0) as [beh SB].
+  exists beh; econstructor; eauto.
+(* 2. Initial state is undefined *)
+  exists (Goes_wrong E0). apply program_goes_initially_wrong.
+  intros. eapply not_ex_all_not; eauto.
+Qed.
+
 End PROGRAM_BEHAVIORS.
+
+(** * Forward simulations and program behaviors *)
+
+Section FORWARD_SIMULATIONS.
+
+Context L1 L2 index order match_states (S: fsim_properties L1 L2 index order match_states).
+
+Lemma forward_simulation_state_behaves:
+  forall i s1 s2 beh1,
+  match_states i s1 s2 -> state_behaves L1 s1 beh1 ->
+  exists beh2, state_behaves L2 s2 beh2 /\ behavior_improves beh1 beh2.
+Proof.
+  intros. inv H0.
+- (* termination *)
+  exploit simulation_star; eauto. intros [i' [s2' [A B]]].
+  exists (Terminates t); split.
+  econstructor; eauto. eapply fsim_match_final_states; eauto.
+  apply behavior_improves_refl.
+- (* silent divergence *)
+  exploit simulation_star; eauto. intros [i' [s2' [A B]]].
+  exists (Diverges t); split.
+  econstructor; eauto. eapply simulation_forever_silent; eauto.
+  apply behavior_improves_refl.
+- (* reactive divergence *)
+  exists (Reacts T); split.
+  econstructor. eapply simulation_forever_reactive; eauto.
+  apply behavior_improves_refl.
+- (* going wrong *)
+  exploit simulation_star; eauto. intros [i' [s2' [A B]]].
+  destruct (state_behaves_exists L2 s2') as [beh' SB].
+  exists (behavior_app t beh'); split.
+  eapply state_behaves_app; eauto.
+  replace (Goes_wrong t) with (behavior_app t (Goes_wrong E0)).
+  apply behavior_improves_app. apply behavior_improves_bot.
+  simpl. decEq. traceEq.
+Qed.
+
+End FORWARD_SIMULATIONS.
+
+Theorem forward_simulation_behavior_improves:
+  forall L1 L2, forward_simulation L1 L2 ->
+  forall beh1, program_behaves L1 beh1 ->
+  exists beh2, program_behaves L2 beh2 /\ behavior_improves beh1 beh2.
+Proof.
+  intros L1 L2 FS. destruct FS as [init order match_states S]. intros. inv H.
+- (* initial state defined *)
+  exploit (fsim_match_initial_states S); eauto. intros [i [s' [INIT MATCH]]].
+  exploit forward_simulation_state_behaves; eauto. intros [beh2 [A B]].
+  exists beh2; split; auto. econstructor; eauto.
+- (* initial state undefined *)
+  destruct (classic (exists s', initial_state L2 s')).
+  destruct H as [s' INIT].
+  destruct (state_behaves_exists L2 s') as [beh' SB].
+  exists beh'; split. econstructor; eauto. apply behavior_improves_bot.
+  exists (Goes_wrong E0); split.
+  apply program_goes_initially_wrong.
+  intros; red; intros. elim H; exists s; auto.
+  apply behavior_improves_refl.
+Qed.
+
+Corollary forward_simulation_same_safe_behavior:
+  forall L1 L2, forward_simulation L1 L2 ->
+  forall beh,
+  program_behaves L1 beh -> not_wrong beh ->
+  program_behaves L2 beh.
+Proof.
+  intros. exploit forward_simulation_behavior_improves; eauto.
+  intros [beh' [A B]]. destruct B.
+  congruence.
+  destruct H1 as [t [C D]]. subst. contradiction.
+Qed.
